Seems mostly alright for Model.AEAD

src/Model.AEAD.fst
@@ -94,3 +94,45 @@ let encrypt i w nonce aad plain_length plain =
     let iv = NoncePkg?.repr (wgetinfo w).nonce i nonce in
     let p = PlainPkg?.repr (wgetinfo w).plain i plain_length plain in
     Spec.encrypt #a k iv aad p
+
+let rec equal (x y: Seq.seq Spec.uint8): Tot (b:bool { b <==> x `Seq.equal` y }) (decreases (Seq.length x)) =
+  if Seq.length x = 0 && Seq.length y = 0 then
+    true
+  else if Seq.length x = 0 && Seq.length y <> 0 then
+    false
+  else if Seq.length x <> 0 && Seq.length y = 0 then
+    false
+  else
+    let hx = Seq.head x in
+    let hy = Seq.head y in
+    let tx = Seq.tail x in
+    let ty = Seq.tail y in
+    if Lib.RawIntTypes.u8_to_UInt8 hx = Lib.RawIntTypes.u8_to_UInt8 hy && equal tx ty then begin
+      assert (x `Seq.equal` Seq.append (Seq.create 1 hx) tx);
+      assert (y `Seq.equal` Seq.append (Seq.create 1 hy) ty);
+      assert (Seq.index (Seq.create 1 hx) 0 == Seq.index (Seq.create 1 hy) 0);
+      assert (Seq.create 1 hx `Seq.equal` Seq.create 1 hy);
+      true
+    end else
+      false
+
+let decrypt i #w r aad n l c =
+  if is_safe i then
+    let w: model_writer i = w in
+    let log = !*(dsnd w) in
+    match Seq.find_l (nonce_filter n) log with
+    | None -> None
+    | Some (Entry n' aad' #l' p' c') ->
+        assert (n == n');
+        if equal aad aad' && equal c c' && l = l' then
+          Some p'
+        else
+          None
+  else
+    let a = (wgetinfo w).alg in
+    let k: Spec.kv a = wkey w in
+    let iv = NoncePkg?.repr (wgetinfo w).nonce i n in
+    match Spec.decrypt k iv aad c with
+    | None -> None
+    | Some p ->
+        Some ((wgetinfo w).plain.mk i (Seq.length p) p)
